proof/invariant-abstract/ARM_HYP/ArchDetSchedSchedule_AI.thy
@@ -5,7 +5,7 @@
  *)
 
 theory ArchDetSchedSchedule_AI
-imports DetSchedSchedule_AI
+imports DetSchedSchedule_AI ArchVCPU_AI
 begin
 
 context Arch begin global_naming ARM_HYP
